src/Blocks.v
@@ -38,7 +38,6 @@ Record OpInfo `{Monad m} (opType1 opType2 : Set) := {
   opKind      : opType1 -> OpKind;
   opRefs      : opType1 -> seq VarInfo;
   moveOp      : PhysReg -> VarId -> PhysReg -> m (seq opType2);
-  swapOp      : PhysReg -> VarId -> PhysReg -> VarId -> m (seq opType2);
   saveOp      : PhysReg -> VarId -> m (seq opType2);
   restoreOp   : VarId   -> PhysReg -> m (seq opType2);
   applyAllocs : opType1 -> seq (VarId * PhysReg) -> m (seq opType2);
